update

Exercises week 4/21_exercise_sheet.lean
@@ -10,7 +10,7 @@ predicate `α → bool`.
 
 def count {α : Type} (a : α) [decidable_eq α] : list α → ℕ
 | [] := 0
-| (x :: xs) := count xs + 1
+| (x :: xs) := count xs + (if x = a then 1 else 0)
 
 
 
@@ -38,18 +38,31 @@ lemma count_le_length {α : Type} (a : α) [decidable_eq α] :
 | [] := by refl
 | (x :: xs) :=
   calc count a (x :: xs) = count a xs + (if x = a then 1 else 0) :
-    begin repeat{simp[count]}, induction xs, simp[count],  end
+    by refl
   ... ≤ list.length xs + (if x = a then 1 else 0) :
-    sorry
+    begin
+      apply add_le_add_right,
+      simp[count_le_length xs]
+    end
   ... ≤ list.length (x :: xs) :
-    begin repeat{simp[count]}, simp[count_le_length a] end
+    begin 
+      apply add_le_add_left,
+      by_cases (x=a),
+      simp[h, list.length],
+      simp[h, list.length],
+      apply nat.le_add_left
+    end
 
 
 /- Question 2: Removing duplicates -/
 
 /- 2.1. Define a predicate `mem x xs` that returns true if `x` is an element of `xs`. -/
 
--- enter your answer here
+def mem {α: Type} (x: α) [decidable_eq α]: list α → bool 
+| [] := false
+| (xs :: xss) := if (xs = x) then true else mem xss 
+
+#reduce mem 2 [7,1]
 
 /- The above `mem` predicate is not quite as convenient as the predefined `list.mem`, for which
 theorems and a nice notation (infix `∈`) are available, including a proof of decidability. Let's use
@@ -65,12 +78,14 @@ occurrences of `1` is kept.
 
 Hint: One of the two behaviors is easier to implement. -/
 
--- enter your answer here
+def remdumps {α: Type} [decidable_eq α]: list α → list α
+| [] := []
+| (x :: xs) := if list.mem x xs then remdumps xs else x :: remdumps xs
 
 /- 2.3. Test your implementation on more than two input values, using `#reduce` or `#eval`, and put
 the expected value in a comment. -/
 
--- enter your answer here
+#reduce remdumps [2,2,2,3,4,4,4] --Expect 2,3,4
 
 /- Do you find yourself copy-pasting the outcome of `#reduce` into the comment? If so, this defeats
 the point of writing a test. You should first think for yourself of the expected result, write it
@@ -79,11 +94,13 @@ down, and then compare the actual result with it. -/
 /- 2.4. Define a function `remdups_adj` that compresses adjacent duplicates. For example, it would
 leave `[1, 2, 1, 3]` unchanged but compress `[1, 1, 2, 2, 2, 1, 3, 3]` to `[1, 2, 1, 3]`. -/
 
--- enter your definition here
+def remdumps_adj {α: Type} [decidable_eq α]: list α → list α
+| [] := []
+| (x :: xs) := if list.mem x xs && (list.take (list.length xs - list.length(remdumps_adj xs)) = x then remdumps_adj xs else x :: remdumps_adj xs
 
 /- 2.5. Test your implementation on the same values as you used for question 2.3. -/
 
--- enter your answer here
+#reduce remdumps_adj [2,2,2,3,4,3,4]
 
 /- Do the tests detect any difference in behavior between `remdups` and `remdups_adj`? If the answer
 is no, this is a strong indication that your tests were incomplete to start with. -/
@@ -94,12 +111,39 @@ Hint: Use `by_cases` to distinguish between the case where a given element is ke
 where it is removed. -/
 
 @[simp] lemma mem_remdups {α : Type} (a : α) [decidable_eq α] :
-  ∀xs : list α, a ∈ remdups xs ↔ a ∈ xs
-:= sorry
+  ∀xs : list α, a ∈ remdumps xs ↔ a ∈ xs
+| [] := by refl
+| (x :: xs) := begin simp[remdumps], by_cases list.mem x xs, { simp [h, mem_remdups xs],
+      apply iff.intro,
+      { intro, apply or.intro_right, assumption },
+      { intro hor,
+        apply hor.elim,
+        { intro a_eq_x, rw a_eq_x, assumption },
+        { intro, assumption } } },
+    { simp [h, mem_remdups xs] } end
+
+-- begin
+-- intro xs,
+-- apply iff.intro,
+-- intro l,
+-- by_cases a ∈ xs,
+-- assumption,
+-- cases xs,
+-- simp,
+-- apply l,
+
+
+
+-- end
 
 /- 2.7. State and prove that `remdups_adj` does not influence the behavior of `list.mem`. -/
-
--- enter your answer here
+lemma test {α: Type} (xs: list α) (x: α) [decidable_eq α]: remdumps_adj xs = xs :=
+begin
+cases xs,
+refl,
+simp[remdumps_adj],
+by_cases 
+end
 
 /- 2.8. State and prove that `remdups` is idempotent (i.e., that applying it twice has the same
 effect as applying it only once). -/
