Project/mergesort.lean
@@ -1,15 +1,16 @@
+def new_list_sizeof : has_sizeof (list ℕ) := ⟨list.length⟩
+local attribute [instance, priority 100000] new_list_sizeof
+
+-- def insert {α: Type} (i: Prop) [decidable i] :list α → list α
+-- | [] := [i]
+-- | (x :: xs) := if x >= i then i :: (x :: xs) else x :: insert i xs
+
+-- -- def insertionSort {α: Type}: list α → ℕ → list α
+-- -- | [] 0 := []
+-- -- | (x :: xs) n := 
 
 
-def insert {α: Type} (i: α) :list α → list α
-| [] := [i]
-| (x :: xs) := if x >= i then i :: (x :: xs) else x :: insert i xs
-
-def insertionSort {α: Type}: list α → ℕ → list α
-| [] 0 := []
-| (x :: xs) n := 
-
-
-
+-- Creating definitions for the mergesort
 def fhalf {α: Type} (xs: list α): list α := list.take (list.length xs/2) xs
 
 def sndhalf {α: Type} (xs: list α): list α := list.drop (list.length xs/2) xs
@@ -18,63 +19,153 @@ def sndhalf {α: Type} (xs: list α): list α := list.drop (list.length xs/2) xs
 #reduce sndhalf [1,2,3,4,5,6]
 
 
-def merge {α: Type}: list α → list α → list α
+-- Definition of the merge (sorting all in one go)
+def merge : list ℕ → list ℕ → list ℕ
    | xs [] := xs
    | [] ys := ys
-   | (x :: xs) (y :: ys) := x :: y :: merge xs ys
-      
-#reduce merge [2,3,7]  [2,3,4]
+   | (x :: xs) (y :: ys) := if x < y then x :: merge xs (y :: ys) else y :: merge (x :: xs) ys
+
+-- Standard definitions for proving with merge later
+def reverse {α : Type} : list α → list α
+| []        := []
+| (x :: xs) := reverse xs ++ [x]
+
+def concat {α: Type}: list (list α) → list α
+| [] := []
+| (xs :: xss) := xs ++ concat xss
+
+      -- then x :: y :: merge xs ys
+
+-- Testing the merge
+#reduce merge [2,23,1] [22,6,7]    --Expecting: [2, 2, 3, 3, 4, 7]
+#reduce merge [22,6,7] [2,23,1]     --Expecting: [2, 2, 3, 3, 4, 7]
+#reduce merge [2,3,4] [2,3,7]    --Expecting: [2, 2, 3, 3, 4, 7]
 
 
-def mergesort {α: Type} (a: α): list α → list α
+#reduce reverse(reverse(merge [2,3,7] [2,3,4]))
+
+-- def mergepairs : list(list ℕ) → list(list ℕ)
+-- | (xs :: xss :: xsss) := merge xs xss :: mergepairs xsss
+-- | xsss := xsss
+
+-- def merge' : list(list ℕ) → list(list ℕ) 
+-- | [] := []
+-- | [x] := [x]
+-- | xs := merge' (mergepairs xs)
+
+
+
+
+def mergesort : list ℕ → list ℕ 
    | [] := []
    | [a] := [a]
-   | (x::xs) :=  merge (mergesort (fhalf xs)) (mergesort (sndhalf xs)) 
+   | (xs) := 
+      have list.sizeof (fhalf xs) < list.sizeof xs, from begin simp[fhalf], cases xs, simp,  end,
+      have list.sizeof (sndhalf xs) < list.sizeof xs, from begin simp[sndhalf], simp [fhalf]  at this, cases xs, simp, simp[] end,
+   merge (mergesort (fhalf xs)) (mergesort (sndhalf xs))
+
+-- def mergesortt : list ℕ → list ℕ     
+-- | [] := []    
+-- | [a] := [a]  
+-- | (x::xs) := 
+--   have list.sizeof (fhalf xs) < x + (1 + list.sizeof xs), from begin induction x, simp, simp[fhalf], cases xs, simp, assumption end,
+--   have list.sizeof (sndhalf xs) < x + (1 + list.sizeof xs), from sorry,
+--   merge (mergesort (fhalf xs)) (mergesort (sndhalf xs))
+
+#reduce mergesort [10,2,1,2,3] 
 
 
-#reduce mergesort [2,3,4,9,2,1]
 
-lemma merge_nil {α : Type} : ∀(n : list α), merge ([] : list α) n  = n :=
+
+
+
+
+
+-- Proving the merge definition instead of the mergesort as it includes the merge defenition. 
+
+
+-- Beginning with creating standard lemmas
+lemma reverse_concat {α : Type} : ∀(x : α) (xs ys : list α), reverse xs ++ x :: reverse ys = reverse xs ++ reverse ys ++ [x]  := sorry
+lemma concat_append {α : Type} : ∀(x : α) (xs : list α), xs ++ [x] = x :: xs := sorry
+
+
+-- Proving the reverse definitions which will also partially be applied to the merge definition
+lemma reverse_append {α : Type} : ∀xs ys : list α, reverse (xs ++ ys)  = reverse xs ++ reverse ys :=
+begin
+intros xs ys,
+induction xs,
+simp,
+simp[reverse],
+simp[concat],
+simp[reverse],
+rw[xs_ih],
+simp[reverse],
+simp[reverse_concat]
+end
+
+
+lemma reverse_append_nil : ∀{α:Type} (xs:list α) (x:α), reverse (x::xs) = reverse xs ++ ( x :: list.nil) :=
+begin
+intros x xs x,
+simp[reverse]
+end
+
+lemma reverse_reverse : ∀(n: list ℕ), reverse (reverse n) = n :=
+begin
+intro n,
+induction n,
+refl,
+simp[reverse],
+simp[reverse_append],
+simp[reverse],
+rw[n_ih],
+simp[concat_append]
+end
+
+
+-- Proving merge properties
+lemma merge_nil: ∀(n : list ℕ), merge ([] : list ℕ) n  = n :=
 begin
 intro n,
 cases n,
 repeat {simp[merge]}
 end
 
-lemma merge_comm {α : Type} : ∀(n : list α),∀(a : list α), merge n a = merge a n :=
+lemma nil_merge: ∀(n : list ℕ), merge n ([] : list ℕ)  = n :=
 begin
-intros a n,
-induction a,
+intro n,
+cases n,
+repeat {simp[merge]}
+end
+
+
+lemma merge_reverse_reverse : ∀(n m: list ℕ), reverse(reverse(merge n m)) = merge n m :=
+begin
+intros n m,
 induction n,
-simp[merge],
-simp[merge],
-
-
+simp[merge_nil],
+simp[reverse_reverse],
+sorry
 end
 
-lemma test {α : Type} : ∀(n : list α),∀(a : list α), merge (n ++ a) = merge (a ++ n) :=
+-- Seems obvious, but can't seem to prove the ite..
+lemma merge_cons: ∀(xs xss : list ℕ), ∀(x: ℕ),  merge xs (x::xss) = merge (x::xss) xs := 
 begin
-intros a n,
-induction a,
+intros xs xss x,
+induction xs,
+simp[nil_merge, merge_nil],
 simp[merge],
-simp[merge],
-
+sorry
 end
 
-section sort
- universe u
-  parameters {α : Type u} (r : α → α → Prop) [decidable_rel r]
-   local infix `=>` : 50 := r 
-   def ordered_insert (a : α) : list α → list α 
-   | [] := [a] 
-   | (b :: l) := if a => b then a :: (b :: l) else b :: ordered_insert l 
-   
-   def insertion_sort : list α → list α 
-   | [] := [] 
-   | (b :: l) := ordered_insert b (insertion_sort l)
+lemma comm_merge : ∀(n m: list ℕ), merge m n = merge n m:=
+begin
+intros n m,
+induction n,
+simp[merge_nil, nil_merge],
+simp[merge_cons]
+end
 
-   def quicksort {α: Type} (a: α) : list α → list α
-| [] := []
-| (x :: xs) := if quicksort (list.filter < a, xs) then  ++ [x] else ++ quicksort (list.filter (>= x) xs)
 
-end sort
+
+
