Project/test.lean
@@ -6,16 +6,24 @@ def map {α β : Type} (f : α → β) : list α → list β |
  [] := [] |
   (x :: xs) := f x :: map xs
 
-lemma map_concat {α β : Type} (f : α → β) : ∀xss : list (list α), map f (concat xss) = concat (map (map f) xss)
-| [] := by refl
-| (xs :: xss) := begin rw[concat], rw[map], rw[concat], rw[<-map_concat xss], end
 
-def reverseList {α: Type}: list α → list α
+def reverse {α: Type}: list α → list α
 | [] := []
-| (x::xs) := reverseList xs ++ [x]
+| (x::xs) := reverse xs ++ [x]
 
 
-#reduce reverseList [2,3,4,5]
+lemma concat_snoc {α : Type} : ∀(xs : list α) (xss : list (list α)), concat (xss ++ [xs]) = concat xss ++ xs:=sorry
+lemma reverse_append {α : Type} : ∀xs ys : list α, reverse (xs ++ ys) = reverse xs ++ reverse ys := sorry
+
+lemma reverse_concat {α : Type} : ∀xss : list (list α), reverse (concat xss) = concat (reverse (map reverse xss))
+| [] := by refl
+| (x :: xs) := begin simp[concat], simp[map], simp[reverse], simp[reverse_append], simp[concat_snoc], rw[reverse_concat xs]  end
+
+
+inductive sorted: list ℕ → Prop
+| nil : sorted []
+| single {n: ℕ} : sorted [n]
+| largertwo {x y: ℕ} {xs: list ℕ} (xy: x <= y) (yxs: sorted (y :: xs)) : sorted (x :: y :: xs)
 -- intro xss,
 -- induction xss,
 -- refl,
@@ -23,3 +31,120 @@ def reverseList {α: Type}: list α → list α
 -- simp[concat],
 -- rw[<-xss_ih],
 
+example : sorted [] := sorted.nil
+
+example : sorted [2] := sorted.single
+
+example : sorted [3, 5] := begin apply sorted.largertwo, trivial, sorted.single  end
+example : sorted [7, 9, 9, 11] := begin apply repeat{sorted.largertwo}, trivial, end
+
+
+
+inductive program (σ : Type) : Type 
+| skip {} : program 
+| assign : (σ → σ) → program 
+| seq : program → program → program 
+| ite : (σ → Prop) → program → program → program 
+| while : (σ → Prop) → program → program
+
+def program_equiv (p1 p2 : program σ) : Prop :=
+ ∀s t, (p1, s) =⇒ t ↔ (p2, s) =⇒ t 
+
+
+inductive finite {α: Type}: set α → Prop
+| empty: finite ∅
+| single {a: α}: finite(insert a ∅)
+| both_fin {A B: set α} (fin_A: finite A) (fin_B: finite B): finite (A ∪ B)
+
+lemma finite.union {α : Type} : ∀A B : set α, finite A → finite B → finite (A ∪ B) :=
+begin
+intros A B,
+intros finA finB,
+apply finite.both_fin,
+assumption,
+assumption
+end
+
+instance fin_set.rel (α : Type) : setoid (list α) := 
+{ r := λxs ys, ∀x, x ∈ xs ↔ x ∈ ys,
+ iseqv := r x x 
+  }
+
+lemma isreflective {α: Type} (xs: list α): xs = xs := sorry
+
+
+
+ 
+namespace v1
+
+
+
+def concat {α: Type}: list (list α) → list α
+| [] := []
+| (xs :: xss) := xs ++ concat xss
+
+def reverse {α: Type}: list α → list α
+| [] := []
+| (x :: xs) := reverse xs ++ [x]
+
+#reduce reverse [2,3,4]
+
+def map {α β: Type} (f: α → β): list α → list β
+| [] := []
+| (x :: xs) := f x :: map xs
+
+lemma map_append {α: Type}: ∀xs ys : list α, map f (xs ++ ys) = (map xs) ++ (map ys)
+#reduce  map 2 [2,3,4]
+
+
+lemma map_concat {α β : Type} (f : α → β) : ∀xss : list (list α), map f (concat xss) = concat (map (map f) xss)
+| [] := by refl
+| (x :: xss) := begin simp[concat], simp[map], simp[concat], rw[<-map_concat xss], induction xss, simp[concat], simp[map], simp[map_concat], simp[map], simp[concat],  end
+
+lemma concat_snoc {α : Type} : ∀(xs : list α) (xss : list (list α)), concat (xss ++ [xs]) = concat xss ++ xs := sorry
+
+lemma reverse_append {α : Type} : ∀xs ys : list α, reverse (xs ++ ys) = reverse xs ++ reverse ys := sorry
+
+lemma reverse_concat {α : Type} : ∀xss : list (list α), reverse (concat xss) = concat (reverse (map reverse xss))
+| [] := by refl
+| (x :: xss) := begin simp[concat], simp[map], simp[reverse], simp[concat_snoc],simp[reverse_append], rw[reverse_concat xss], simp end
+
+inductive sorted: list ℕ → Prop
+| empty : sorted []
+| any_list {a: ℕ}: sorted [a]
+| greater_two {xs: list ℕ} {x y: ℕ} (xsmallery: x <= y) (sxy: sorted (y :: xs)) : sorted (x :: y :: xs)
+
+example : sorted [] := sorted.empty
+example : sorted [2] := sorted.any_list
+example : sorted [3, 5] := begin apply sorted.greater_two, apply trivial, apply sorted.any_list end
+example : sorted [7, 9, 9, 11] := begin apply sorted.greater_two, apply trivial, apply sorted.greater_two...end
+example : ¬ sorted [17, 13] := begin assume s : sorted [17,13],begin have 17 <= 13 := match s with sorted.greater_two xy yxs := xy end end
+
+-- inductive finite {α: Type} : set α → Prop
+-- | empty : finite ∅
+-- | finite_set {a: α} {A: set α} (finA : finite A) : finite ({a} ∪ A)
+
+inductive finite {α: Type} : set α → Prop
+| empty : finite ∅
+| singleton {a: α} : finite (insert a ∅)
+| ABFinite {finiteA finiteB: set α} (afinite: finite finiteA) (bfinite: finite finiteB) : finite (finiteA ∪ finiteB)
+
+lemma finite.union {α : Type} :
+∀A B : set α, finite A → finite B → finite (A ∪ B) :=
+begin
+intros A B,
+intros finiteA finiteB,
+apply finite.ABFinite,
+repeat{assumption}
+end
+
+
+lemma refleciver {α: Type} (xs: list α): xs = xs := by refl
+
+lemma symmetric {α: Type} (xs ys: list α): xs → ys = ys → xs := sorry
+
+lemma transitive {α: Type} (xs ys zs: list α): xs → ys ∧ ys → zs = xs → zs := sorry
+ 
+def fin_empty {α : Type} (a: α) : fin_set α := [[a]] 
+
+end v1
